include/s2n-bignum-c89.h
@@ -477,6 +477,11 @@ extern void bignum_montmul_p384_alt (uint64_t z[6], uint64_t x[6], uint64_t y[6]
 extern void bignum_montmul_p521 (uint64_t z[9], uint64_t x[9], uint64_t y[9]);
 extern void bignum_montmul_p521_alt (uint64_t z[9], uint64_t x[9], uint64_t y[9]);
 
+/*  Montgomery multiply, z := (x * y / 2^256) mod p_sm2 */
+/*  Inputs x[4], y[4]; output z[4] */
+extern void bignum_montmul_sm2 (uint64_t z[4], uint64_t x[4], uint64_t y[4]);
+extern void bignum_montmul_sm2_alt (uint64_t z[4], uint64_t x[4], uint64_t y[4]);
+
 /*  Montgomery reduce, z := (x' / 2^{64p}) MOD m */
 /*  Inputs x[n], m[k], p; output z[k] */
 extern void bignum_montredc (uint64_t k, uint64_t *z, uint64_t n, uint64_t *x, uint64_t *m, uint64_t p);
@@ -504,6 +509,11 @@ extern void bignum_montsqr_p384_alt (uint64_t z[6], uint64_t x[6]);
 /*  Input x[9]; output z[9] */
 extern void bignum_montsqr_p521 (uint64_t z[9], uint64_t x[9]);
 extern void bignum_montsqr_p521_alt (uint64_t z[9], uint64_t x[9]);
+
+/*  Montgomery square, z := (x^2 / 2^256) mod p_sm2 */
+/*  Input x[4]; output z[4] */
+extern void bignum_montsqr_sm2 (uint64_t z[4], uint64_t x[4]);
+extern void bignum_montsqr_sm2_alt (uint64_t z[4], uint64_t x[4]);
 
 /*  Multiply z := x * y */
 /*  Inputs x[m], y[n]; output z[k] */
