arm/proofs/bignum_montmul_sm2_alt.ml
@@ -4,14 +4,14 @@
  *)
 
 (* ========================================================================= *)
-(* Montgomery multiplication modulo p_256.                                   *)
+(* Montgomery multiplication modulo p_sm2.                                   *)
 (* ========================================================================= *)
 
-(**** print_literal_from_elf "arm/p256/bignum_montmul_p256_alt.o";;
+(**** print_literal_from_elf "arm/sm2/bignum_montmul_sm2_alt.o";;
  ****)
 
-let bignum_montmul_p256_alt_mc =
-  define_assert_from_elf "bignum_montmul_p256_alt_mc" "arm/p256/bignum_montmul_p256_alt.o"
+let bignum_montmul_sm2_alt_mc =
+  define_assert_from_elf "bignum_montmul_sm2_alt_mc" "arm/sm2/bignum_montmul_sm2_alt.o"
 [
   0xa9401023;       (* arm_LDP X3 X4 X1 (Immediate_Offset (iword (&0))) *)
   0xa9402047;       (* arm_LDP X7 X8 X2 (Immediate_Offset (iword (&0))) *)
@@ -81,47 +81,47 @@ let bignum_montmul_p256_alt_mc =
   0xba0b0084;       (* arm_ADCS X4 X4 X11 *)
   0x9a1f00a5;       (* arm_ADC X5 X5 XZR *)
   0xd3607d8b;       (* arm_LSL X11 X12 32 *)
-  0xeb0b0188;       (* arm_SUBS X8 X12 X11 *)
   0xd360fd86;       (* arm_LSR X6 X12 32 *)
+  0xeb0c0168;       (* arm_SUBS X8 X11 X12 *)
+  0xda1f00c7;       (* arm_SBC X7 X6 XZR *)
+  0xeb0801ad;       (* arm_SUBS X13 X13 X8 *)
+  0xfa0701ce;       (* arm_SBCS X14 X14 X7 *)
+  0xfa0b01ef;       (* arm_SBCS X15 X15 X11 *)
   0xda06018c;       (* arm_SBC X12 X12 X6 *)
-  0xab0b01ad;       (* arm_ADDS X13 X13 X11 *)
-  0xba0601ce;       (* arm_ADCS X14 X14 X6 *)
-  0xba0801ef;       (* arm_ADCS X15 X15 X8 *)
-  0x9a1f018c;       (* arm_ADC X12 X12 XZR *)
   0xd3607dab;       (* arm_LSL X11 X13 32 *)
-  0xeb0b01a8;       (* arm_SUBS X8 X13 X11 *)
   0xd360fda6;       (* arm_LSR X6 X13 32 *)
+  0xeb0d0168;       (* arm_SUBS X8 X11 X13 *)
+  0xda1f00c7;       (* arm_SBC X7 X6 XZR *)
+  0xeb0801ce;       (* arm_SUBS X14 X14 X8 *)
+  0xfa0701ef;       (* arm_SBCS X15 X15 X7 *)
+  0xfa0b018c;       (* arm_SBCS X12 X12 X11 *)
   0xda0601ad;       (* arm_SBC X13 X13 X6 *)
-  0xab0b01ce;       (* arm_ADDS X14 X14 X11 *)
-  0xba0601ef;       (* arm_ADCS X15 X15 X6 *)
-  0xba08018c;       (* arm_ADCS X12 X12 X8 *)
-  0x9a1f01ad;       (* arm_ADC X13 X13 XZR *)
   0xd3607dcb;       (* arm_LSL X11 X14 32 *)
-  0xeb0b01c8;       (* arm_SUBS X8 X14 X11 *)
   0xd360fdc6;       (* arm_LSR X6 X14 32 *)
+  0xeb0e0168;       (* arm_SUBS X8 X11 X14 *)
+  0xda1f00c7;       (* arm_SBC X7 X6 XZR *)
+  0xeb0801ef;       (* arm_SUBS X15 X15 X8 *)
+  0xfa07018c;       (* arm_SBCS X12 X12 X7 *)
+  0xfa0b01ad;       (* arm_SBCS X13 X13 X11 *)
   0xda0601ce;       (* arm_SBC X14 X14 X6 *)
-  0xab0b01ef;       (* arm_ADDS X15 X15 X11 *)
-  0xba06018c;       (* arm_ADCS X12 X12 X6 *)
-  0xba0801ad;       (* arm_ADCS X13 X13 X8 *)
-  0x9a1f01ce;       (* arm_ADC X14 X14 XZR *)
   0xd3607deb;       (* arm_LSL X11 X15 32 *)
-  0xeb0b01e8;       (* arm_SUBS X8 X15 X11 *)
   0xd360fde6;       (* arm_LSR X6 X15 32 *)
+  0xeb0f0168;       (* arm_SUBS X8 X11 X15 *)
+  0xda1f00c7;       (* arm_SBC X7 X6 XZR *)
+  0xeb08018c;       (* arm_SUBS X12 X12 X8 *)
+  0xfa0701ad;       (* arm_SBCS X13 X13 X7 *)
+  0xfa0b01ce;       (* arm_SBCS X14 X14 X11 *)
   0xda0601ef;       (* arm_SBC X15 X15 X6 *)
-  0xab0b018c;       (* arm_ADDS X12 X12 X11 *)
-  0xba0601ad;       (* arm_ADCS X13 X13 X6 *)
-  0xba0801ce;       (* arm_ADCS X14 X14 X8 *)
-  0x9a1f01ef;       (* arm_ADC X15 X15 XZR *)
   0xab10018c;       (* arm_ADDS X12 X12 X16 *)
   0xba0301ad;       (* arm_ADCS X13 X13 X3 *)
   0xba0401ce;       (* arm_ADCS X14 X14 X4 *)
   0xba0501ef;       (* arm_ADCS X15 X15 X5 *)
   0x9a9f37e8;       (* arm_CSET X8 Condition_CS *)
-  0xb2407feb;       (* arm_MOV X11 (rvalue (word 4294967295)) *)
-  0xb26083e6;       (* arm_MOV X6 (rvalue (word 18446744069414584321)) *)
+  0xb2607feb;       (* arm_MOV X11 (rvalue (word 18446744069414584320)) *)
+  0x92c00026;       (* arm_MOVN X6 (word 1) 32 *)
   0xb1000590;       (* arm_ADDS X16 X12 (rvalue (word 1)) *)
   0xfa0b01a3;       (* arm_SBCS X3 X13 X11 *)
-  0xfa1f01c4;       (* arm_SBCS X4 X14 XZR *)
+  0xba1f01c4;       (* arm_ADCS X4 X14 XZR *)
   0xfa0601e5;       (* arm_SBCS X5 X15 X6 *)
   0xfa1f011f;       (* arm_SBCS XZR X8 XZR *)
   0x9a90318c;       (* arm_CSEL X12 X12 X16 Condition_CC *)
@@ -133,27 +133,27 @@ let bignum_montmul_p256_alt_mc =
   0xd65f03c0        (* arm_RET X30 *)
 ];;
 
-let BIGNUM_MONTMUL_P256_ALT_EXEC = ARM_MK_EXEC_RULE bignum_montmul_p256_alt_mc;;
+let BIGNUM_MONTMUL_SM2_ALT_EXEC = ARM_MK_EXEC_RULE bignum_montmul_sm2_alt_mc;;
 
 (* ------------------------------------------------------------------------- *)
 (* Proof.                                                                    *)
 (* ------------------------------------------------------------------------- *)
 
-let p_256 = new_definition `p_256 = 115792089210356248762697446949407573530086143415290314195533631308867097853951`;;
+let p_sm2 = new_definition `p_sm2 = 0xFFFFFFFEFFFFFFFFFFFFFFFFFFFFFFFFFFFFFFFF00000000FFFFFFFFFFFFFFFF`;;
 
-let BIGNUM_MONTMUL_P256_ALT_CORRECT = time prove
+let BIGNUM_MONTMUL_SM2_ALT_CORRECT = time prove
  (`!z x y a b pc.
         nonoverlapping (word pc,0x1d8) (z,8 * 4)
         ==> ensures arm
-             (\s. aligned_bytes_loaded s (word pc) bignum_montmul_p256_alt_mc /\
+             (\s. aligned_bytes_loaded s (word pc) bignum_montmul_sm2_alt_mc /\
                   read PC s = word pc /\
                   C_ARGUMENTS [z; x; y] s /\
                   bignum_from_memory (x,4) s = a /\
                   bignum_from_memory (y,4) s = b)
              (\s. read PC s = word (pc + 0x1d4) /\
-                  (a * b <= 2 EXP 256 * p_256
+                  (a * b <= 2 EXP 256 * p_sm2
                    ==> bignum_from_memory (z,4) s =
-                       (inverse_mod p_256 (2 EXP 256) * a * b) MOD p_256))
+                       (inverse_mod p_sm2 (2 EXP 256) * a * b) MOD p_sm2))
              (MAYCHANGE [PC; X3; X4; X5; X6; X7; X8; X9; X10; X11; X12;
                          X13; X14; X15; X16] ,,
               MAYCHANGE [memory :> bytes(z,8 * 4)] ,,
@@ -163,24 +163,24 @@ let BIGNUM_MONTMUL_P256_ALT_CORRECT = time prove
   REWRITE_TAC[C_ARGUMENTS; C_RETURN; SOME_FLAGS; NONOVERLAPPING_CLAUSES] THEN
   DISCH_THEN(REPEAT_TCL CONJUNCTS_THEN ASSUME_TAC) THEN
 
-  (*** Globalize the a * b <= 2 EXP 256 * p_256  assumption ***)
+  (*** Globalize the a * b <= 2 EXP 256 * p_sm2  assumption ***)
 
-  ASM_CASES_TAC `a * b <= 2 EXP 256 * p_256` THENL
-   [ASM_REWRITE_TAC[]; ARM_SIM_TAC BIGNUM_MONTMUL_P256_ALT_EXEC (1--117)] THEN
+  ASM_CASES_TAC `a * b <= 2 EXP 256 * p_sm2` THENL
+   [ASM_REWRITE_TAC[]; ARM_SIM_TAC BIGNUM_MONTMUL_SM2_ALT_EXEC (1--117)] THEN
   ENSURES_INIT_TAC "s0" THEN
   BIGNUM_DIGITIZE_TAC "x_" `bignum_from_memory (x,4) s0` THEN
   BIGNUM_DIGITIZE_TAC "y_" `bignum_from_memory (y,4) s0` THEN
 
   (*** Simulate the core pre-reduced result accumulation ***)
 
-  ARM_ACCSTEPS_TAC BIGNUM_MONTMUL_P256_ALT_EXEC (1--104) (1--104) THEN
+  ARM_ACCSTEPS_TAC BIGNUM_MONTMUL_SM2_ALT_EXEC (1--104) (1--104) THEN
   RULE_ASSUM_TAC(REWRITE_RULE[WORD_UNMASK_64]) THEN
   ABBREV_TAC
    `t = bignum_of_wordlist
           [sum_s100; sum_s101; sum_s102; sum_s103;
            word(bitval carry_s103)]` THEN
   SUBGOAL_THEN
-   `t < 2 * p_256 /\ (2 EXP 256 * t == a * b) (mod p_256)`
+   `t < 2 * p_sm2 /\ (2 EXP 256 * t == a * b) (mod p_sm2)`
   STRIP_ASSUME_TAC THENL
    [ACCUMULATOR_POP_ASSUM_LIST
      (STRIP_ASSUME_TAC o end_itlist CONJ o DECARRY_RULE) THEN
@@ -190,9 +190,9 @@ let BIGNUM_MONTMUL_P256_ALT_CORRECT = time prove
          ==> 2 EXP 256 * t < ab + 2 EXP 256 * p ==> t < 2 * p`)) THEN
       MAP_EVERY EXPAND_TAC ["a"; "b"; "t"] THEN
       REWRITE_TAC[GSYM REAL_OF_NUM_CLAUSES; bignum_of_wordlist] THEN
-      REWRITE_TAC[p_256; REAL_ARITH `a:real < b + c <=> a - b < c`] THEN
+      REWRITE_TAC[p_sm2; REAL_ARITH `a:real < b + c <=> a - b < c`] THEN
       ASM_REWRITE_TAC[VAL_WORD_BITVAL] THEN BOUNDER_TAC[];
-      REWRITE_TAC[REAL_CONGRUENCE; p_256] THEN CONV_TAC NUM_REDUCE_CONV THEN
+      REWRITE_TAC[REAL_CONGRUENCE; p_sm2] THEN CONV_TAC NUM_REDUCE_CONV THEN
       MAP_EVERY EXPAND_TAC ["a"; "b"; "t"] THEN
       REWRITE_TAC[GSYM REAL_OF_NUM_CLAUSES; bignum_of_wordlist] THEN
       ASM_REWRITE_TAC[VAL_WORD_BITVAL] THEN REAL_INTEGER_TAC];
@@ -200,83 +200,83 @@ let BIGNUM_MONTMUL_P256_ALT_CORRECT = time prove
 
   (*** Final correction stage ***)
 
-  ARM_ACCSTEPS_TAC BIGNUM_MONTMUL_P256_ALT_EXEC (107--111) (105--117) THEN
+  ARM_ACCSTEPS_TAC BIGNUM_MONTMUL_SM2_ALT_EXEC (107--111) (105--117) THEN
   RULE_ASSUM_TAC(REWRITE_RULE
    [GSYM WORD_BITVAL; COND_SWAP; REAL_BITVAL_NOT]) THEN
   ENSURES_FINAL_STATE_TAC THEN ASM_REWRITE_TAC[] THEN
   CONV_TAC(LAND_CONV BIGNUM_EXPAND_CONV) THEN ASM_REWRITE_TAC[] THEN
-  TRANS_TAC EQ_TRANS `t MOD p_256` THEN CONJ_TAC THENL
+  TRANS_TAC EQ_TRANS `t MOD p_sm2` THEN CONJ_TAC THENL
    [ALL_TAC;
     REWRITE_TAC[GSYM CONG] THEN FIRST_X_ASSUM(MATCH_MP_TAC o MATCH_MP
      (NUMBER_RULE
        `(e * t == a * b) (mod p)
         ==> (e * i == 1) (mod p) ==> (t == i * a * b) (mod p)`)) THEN
     REWRITE_TAC[INVERSE_MOD_RMUL_EQ; COPRIME_REXP; COPRIME_2] THEN
-    REWRITE_TAC[p_256] THEN CONV_TAC NUM_REDUCE_CONV] THEN
+    REWRITE_TAC[p_sm2] THEN CONV_TAC NUM_REDUCE_CONV] THEN
   CONV_TAC SYM_CONV THEN MATCH_MP_TAC EQUAL_FROM_CONGRUENT_MOD_MOD THEN
   MAP_EVERY EXISTS_TAC
-   [`256`; `if t < p_256 then &t:real else &t - &p_256`] THEN
+   [`256`; `if t < p_sm2 then &t:real else &t - &p_sm2`] THEN
   REPEAT CONJ_TAC THENL
    [REWRITE_TAC[GSYM REAL_OF_NUM_CLAUSES] THEN BOUNDER_TAC[];
-    REWRITE_TAC[p_256] THEN ARITH_TAC;
-    REWRITE_TAC[p_256] THEN ARITH_TAC;
+    REWRITE_TAC[p_sm2] THEN ARITH_TAC;
+    REWRITE_TAC[p_sm2] THEN ARITH_TAC;
     ALL_TAC;
     ASM_SIMP_TAC[MOD_CASES] THEN
     GEN_REWRITE_TAC LAND_CONV [COND_RAND] THEN
     SIMP_TAC[REAL_OF_NUM_SUB; GSYM NOT_LT]] THEN
-  SUBGOAL_THEN `carry_s111 <=> t < p_256` SUBST_ALL_TAC THENL
+  SUBGOAL_THEN `carry_s111 <=> t < p_sm2` SUBST_ALL_TAC THENL
    [MATCH_MP_TAC FLAG_FROM_CARRY_LT THEN EXISTS_TAC `320` THEN
     EXPAND_TAC "t" THEN
-    REWRITE_TAC[p_256; bignum_of_wordlist; GSYM REAL_OF_NUM_CLAUSES] THEN
+    REWRITE_TAC[p_sm2; bignum_of_wordlist; GSYM REAL_OF_NUM_CLAUSES] THEN
     CONV_TAC NUM_REDUCE_CONV THEN REWRITE_TAC[VAL_WORD_BITVAL] THEN
     ACCUMULATOR_POP_ASSUM_LIST(MP_TAC o end_itlist CONJ o DECARRY_RULE) THEN
     DISCH_THEN(fun th -> REWRITE_TAC[th]) THEN BOUNDER_TAC[];
     ALL_TAC] THEN
   COND_CASES_TAC THEN ASM_REWRITE_TAC[] THEN EXPAND_TAC "t" THEN
-  REWRITE_TAC[GSYM REAL_OF_NUM_CLAUSES; bignum_of_wordlist; p_256] THEN
+  REWRITE_TAC[GSYM REAL_OF_NUM_CLAUSES; bignum_of_wordlist; p_sm2] THEN
   ACCUMULATOR_POP_ASSUM_LIST(MP_TAC o end_itlist CONJ o DESUM_RULE) THEN
   ASM_REWRITE_TAC[BITVAL_CLAUSES; VAL_WORD_BITVAL] THEN
   DISCH_THEN(fun th -> REWRITE_TAC[th]) THEN REAL_INTEGER_TAC);;
 
-let BIGNUM_MONTMUL_P256_ALT_SUBROUTINE_CORRECT = time prove
+let BIGNUM_MONTMUL_SM2_ALT_SUBROUTINE_CORRECT = time prove
  (`!z x y a b pc returnaddress.
         nonoverlapping (word pc,0x1d8) (z,8 * 4)
         ==> ensures arm
-             (\s. aligned_bytes_loaded s (word pc) bignum_montmul_p256_alt_mc /\
+             (\s. aligned_bytes_loaded s (word pc) bignum_montmul_sm2_alt_mc /\
                   read PC s = word pc /\
                   read X30 s = returnaddress /\
                   C_ARGUMENTS [z; x; y] s /\
                   bignum_from_memory (x,4) s = a /\
                   bignum_from_memory (y,4) s = b)
              (\s. read PC s = returnaddress /\
-                  (a * b <= 2 EXP 256 * p_256
+                  (a * b <= 2 EXP 256 * p_sm2
                    ==> bignum_from_memory (z,4) s =
-                       (inverse_mod p_256 (2 EXP 256) * a * b) MOD p_256))
+                       (inverse_mod p_sm2 (2 EXP 256) * a * b) MOD p_sm2))
              (MAYCHANGE [PC; X3; X4; X5; X6; X7; X8; X9; X10; X11; X12;
                          X13; X14; X15; X16] ,,
               MAYCHANGE [memory :> bytes(z,8 * 4)] ,,
               MAYCHANGE SOME_FLAGS)`,
-  ARM_ADD_RETURN_NOSTACK_TAC BIGNUM_MONTMUL_P256_ALT_EXEC
-    BIGNUM_MONTMUL_P256_ALT_CORRECT);;
+  ARM_ADD_RETURN_NOSTACK_TAC BIGNUM_MONTMUL_SM2_ALT_EXEC
+    BIGNUM_MONTMUL_SM2_ALT_CORRECT);;
 
 (* ------------------------------------------------------------------------- *)
 (* Show that it also works as "almost-Montgomery" if desired. That is, even  *)
 (* without the further range assumption on inputs we still get a congruence. *)
-(* But the output, still 256 bits, may then not be fully reduced mod p_256.  *)
+(* But the output, still 256 bits, may then not be fully reduced mod p_sm2.  *)
 (* ------------------------------------------------------------------------- *)
 
-let BIGNUM_AMONTMUL_P256_ALT_CORRECT = time prove
+let BIGNUM_AMONTMUL_SM2_ALT_CORRECT = time prove
  (`!z x y a b pc.
         nonoverlapping (word pc,0x1d8) (z,8 * 4)
         ==> ensures arm
-             (\s. aligned_bytes_loaded s (word pc) bignum_montmul_p256_alt_mc /\
+             (\s. aligned_bytes_loaded s (word pc) bignum_montmul_sm2_alt_mc /\
                   read PC s = word pc /\
                   C_ARGUMENTS [z; x; y] s /\
                   bignum_from_memory (x,4) s = a /\
                   bignum_from_memory (y,4) s = b)
              (\s. read PC s = word (pc + 0x1d4) /\
                   (bignum_from_memory (z,4) s ==
-                   inverse_mod p_256 (2 EXP 256) * a * b) (mod p_256))
+                   inverse_mod p_sm2 (2 EXP 256) * a * b) (mod p_sm2))
              (MAYCHANGE [PC; X3; X4; X5; X6; X7; X8; X9; X10; X11; X12;
                          X13; X14; X15; X16] ,,
               MAYCHANGE [memory :> bytes(z,8 * 4)] ,,
@@ -291,14 +291,14 @@ let BIGNUM_AMONTMUL_P256_ALT_CORRECT = time prove
 
   (*** Simulate the core pre-reduced result accumulation ***)
 
-  ARM_ACCSTEPS_TAC BIGNUM_MONTMUL_P256_ALT_EXEC (1--104) (1--104) THEN
+  ARM_ACCSTEPS_TAC BIGNUM_MONTMUL_SM2_ALT_EXEC (1--104) (1--104) THEN
   RULE_ASSUM_TAC(REWRITE_RULE[WORD_UNMASK_64]) THEN
   ABBREV_TAC
    `t = bignum_of_wordlist
           [sum_s100; sum_s101; sum_s102; sum_s103;
            word(bitval carry_s103)]` THEN
   SUBGOAL_THEN
-   `t < 2 EXP 256 + p_256 /\ (2 EXP 256 * t == a * b) (mod p_256)`
+   `t < 2 EXP 256 + p_sm2 /\ (2 EXP 256 * t == a * b) (mod p_sm2)`
   STRIP_ASSUME_TAC THENL
    [ACCUMULATOR_POP_ASSUM_LIST
      (STRIP_ASSUME_TAC o end_itlist CONJ o DECARRY_RULE) THEN
@@ -306,12 +306,12 @@ let BIGNUM_AMONTMUL_P256_ALT_CORRECT = time prove
      [MATCH_MP_TAC(ARITH_RULE
        `2 EXP 256 * t <= (2 EXP 256 - 1) EXP 2 + (2 EXP 256 - 1) * p
         ==> t < 2 EXP 256 + p`) THEN
-      REWRITE_TAC[p_256] THEN CONV_TAC NUM_REDUCE_CONV THEN
+      REWRITE_TAC[p_sm2] THEN CONV_TAC NUM_REDUCE_CONV THEN
       MAP_EVERY EXPAND_TAC ["a"; "b"; "t"] THEN
       REWRITE_TAC[GSYM REAL_OF_NUM_CLAUSES; bignum_of_wordlist] THEN
-      REWRITE_TAC[p_256; REAL_ARITH `a:real < b + c <=> a - b < c`] THEN
+      REWRITE_TAC[p_sm2; REAL_ARITH `a:real < b + c <=> a - b < c`] THEN
       ASM_REWRITE_TAC[VAL_WORD_BITVAL] THEN BOUNDER_TAC[];
-      REWRITE_TAC[REAL_CONGRUENCE; p_256] THEN CONV_TAC NUM_REDUCE_CONV THEN
+      REWRITE_TAC[REAL_CONGRUENCE; p_sm2] THEN CONV_TAC NUM_REDUCE_CONV THEN
       MAP_EVERY EXPAND_TAC ["a"; "b"; "t"] THEN
       REWRITE_TAC[GSYM REAL_OF_NUM_CLAUSES; bignum_of_wordlist] THEN
       ASM_REWRITE_TAC[VAL_WORD_BITVAL] THEN REAL_INTEGER_TAC];
@@ -319,7 +319,7 @@ let BIGNUM_AMONTMUL_P256_ALT_CORRECT = time prove
 
   (*** Final correction stage ***)
 
-  ARM_ACCSTEPS_TAC BIGNUM_MONTMUL_P256_ALT_EXEC (107--111) (105--117) THEN
+  ARM_ACCSTEPS_TAC BIGNUM_MONTMUL_SM2_ALT_EXEC (107--111) (105--117) THEN
   RULE_ASSUM_TAC(REWRITE_RULE
    [GSYM WORD_BITVAL; COND_SWAP; REAL_BITVAL_NOT]) THEN
   ENSURES_FINAL_STATE_TAC THEN ASM_REWRITE_TAC[] THEN
@@ -330,23 +330,23 @@ let BIGNUM_AMONTMUL_P256_ALT_CORRECT = time prove
             ==> (s == i * ab) (mod p)`)) THEN
   REWRITE_TAC[INVERSE_MOD_RMUL_EQ; COPRIME_REXP; COPRIME_2] THEN
   CONJ_TAC THENL
-   [REWRITE_TAC[p_256] THEN CONV_TAC NUM_REDUCE_CONV; ALL_TAC] THEN
-  SUBGOAL_THEN `carry_s111 <=> t < p_256` SUBST_ALL_TAC THENL
+   [REWRITE_TAC[p_sm2] THEN CONV_TAC NUM_REDUCE_CONV; ALL_TAC] THEN
+  SUBGOAL_THEN `carry_s111 <=> t < p_sm2` SUBST_ALL_TAC THENL
    [MATCH_MP_TAC FLAG_FROM_CARRY_LT THEN EXISTS_TAC `320` THEN
     EXPAND_TAC "t" THEN
-    REWRITE_TAC[p_256; bignum_of_wordlist; GSYM REAL_OF_NUM_CLAUSES] THEN
+    REWRITE_TAC[p_sm2; bignum_of_wordlist; GSYM REAL_OF_NUM_CLAUSES] THEN
     CONV_TAC NUM_REDUCE_CONV THEN REWRITE_TAC[VAL_WORD_BITVAL] THEN
     ACCUMULATOR_POP_ASSUM_LIST(MP_TAC o end_itlist CONJ o DECARRY_RULE) THEN
     DISCH_THEN(fun th -> REWRITE_TAC[th]) THEN BOUNDER_TAC[];
     ALL_TAC] THEN
   MATCH_MP_TAC(NUMBER_RULE `!b:num. x + b * p = y ==> (x == y) (mod p)`) THEN
-  EXISTS_TAC `bitval(p_256 <= t)` THEN
+  EXISTS_TAC `bitval(p_sm2 <= t)` THEN
   REWRITE_TAC[GSYM REAL_OF_NUM_CLAUSES] THEN REWRITE_TAC[REAL_OF_NUM_LE] THEN
   ONCE_REWRITE_TAC[REAL_ARITH `a + b:real = c <=> c - b = a`] THEN
   MATCH_MP_TAC EQUAL_FROM_CONGRUENT_REAL THEN
   MAP_EVERY EXISTS_TAC [`256`; `&0:real`] THEN CONJ_TAC THENL
-   [UNDISCH_TAC `t < 2 EXP 256 + p_256` THEN
-    REWRITE_TAC[bitval; p_256; GSYM REAL_OF_NUM_CLAUSES] THEN REAL_ARITH_TAC;
+   [UNDISCH_TAC `t < 2 EXP 256 + p_sm2` THEN
+    REWRITE_TAC[bitval; p_sm2; GSYM REAL_OF_NUM_CLAUSES] THEN REAL_ARITH_TAC;
     REWRITE_TAC[INTEGER_CLOSED]] THEN
   CONJ_TAC THENL
    [CONV_TAC(ONCE_DEPTH_CONV BIGNUM_EXPAND_CONV) THEN
@@ -358,14 +358,14 @@ let BIGNUM_AMONTMUL_P256_ALT_CORRECT = time prove
   ASM_REWRITE_TAC[GSYM REAL_OF_NUM_CLAUSES] THEN
   ACCUMULATOR_POP_ASSUM_LIST (MP_TAC o end_itlist CONJ o DESUM_RULE) THEN
   DISCH_THEN(fun th -> REWRITE_TAC[th]) THEN
-  REWRITE_TAC[BITVAL_CLAUSES; p_256] THEN
+  REWRITE_TAC[BITVAL_CLAUSES; p_sm2] THEN
   CONV_TAC WORD_REDUCE_CONV THEN REAL_INTEGER_TAC);;
 
-let BIGNUM_AMONTMUL_P256_ALT_SUBROUTINE_CORRECT = time prove
+let BIGNUM_AMONTMUL_SM2_ALT_SUBROUTINE_CORRECT = time prove
  (`!z x y a b pc returnaddress.
         nonoverlapping (word pc,0x1d8) (z,8 * 4)
         ==> ensures arm
-             (\s. aligned_bytes_loaded s (word pc) bignum_montmul_p256_alt_mc /\
+             (\s. aligned_bytes_loaded s (word pc) bignum_montmul_sm2_alt_mc /\
                   read PC s = word pc /\
                   read X30 s = returnaddress /\
                   C_ARGUMENTS [z; x; y] s /\
@@ -373,10 +373,10 @@ let BIGNUM_AMONTMUL_P256_ALT_SUBROUTINE_CORRECT = time prove
                   bignum_from_memory (y,4) s = b)
              (\s. read PC s = returnaddress /\
                   (bignum_from_memory (z,4) s ==
-                   inverse_mod p_256 (2 EXP 256) * a * b) (mod p_256))
+                   inverse_mod p_sm2 (2 EXP 256) * a * b) (mod p_sm2))
              (MAYCHANGE [PC; X3; X4; X5; X6; X7; X8; X9; X10; X11; X12;
                          X13; X14; X15; X16] ,,
               MAYCHANGE [memory :> bytes(z,8 * 4)] ,,
               MAYCHANGE SOME_FLAGS)`,
-  ARM_ADD_RETURN_NOSTACK_TAC BIGNUM_MONTMUL_P256_ALT_EXEC
-    BIGNUM_AMONTMUL_P256_ALT_CORRECT);;
+  ARM_ADD_RETURN_NOSTACK_TAC BIGNUM_MONTMUL_SM2_ALT_EXEC
+    BIGNUM_AMONTMUL_SM2_ALT_CORRECT);;
